Update tfind_lo_tfind_armv8_proof.v
final

tfind_lo_tfind_armv8_proof.v
@@ -18,8 +18,8 @@ Definition tfind_exit (t:trace) :=
   end | _ => false end.
 
 (* tfind_lo_tfind_armv8 *)
-
 (* tfind does not corrupt memory. *)
+
 Theorem tfind_preserves_memory:
   forall_endstates tfind_lo_tfind_armv8 (fun _ s _ s' => s V_MEM32 = s' V_MEM32).
 Proof.
@@ -34,78 +34,6 @@ Proof.
   apply noassign_prog_same.
   prove_noassign.
 Qed.
-
-
-Section Invariants.
-
-  Variable sp : N          (* initial stack pointer *).
-  Variable mem : memory    (* initial memory state *).
-  Variable arg1 : N        (* tfind: 1st pointer arg (R_X0)
-                              desired index *).
-  Variable arg2 : N        (* tfind: 2nd pointer arg (R_X1)
-                              root node pointer *).
-  Variable arg3 : N        (* tfind: 3rd pointer arg (R_X2)
-                              address of subroutine*).
-  Variable x20 x21 : N     (* R_X20, R_X21 (callee-save regs) *).
-
-  Definition mem' fbytes := setmem 64 LittleE 40 mem (sp ⊖ 48) fbytes.
-
-  Definition postcondition (s:store) :=
-    ∃ n k fb,
-      s V_MEM64 = mem' fb /\
-      s R_X0 = n /\ (n=0 -> (mem' fb) Ⓑ[arg1+k] = 0).
-  
-  Definition invs T (Inv Post: inv_type T) (NoInv:T) (s:store) (a:addr) : T :=
-    match a with
-    (* tfind entry point *)
-    | 0x100000 => Inv 1 (
-        s R_SP = sp /\ s V_MEM64 = mem /\
-        s R_X0 = arg1 /\ s R_X1 = arg2 /\ s R_X2 = arg3
-      )
-        (* X1 Parameter Validation *)
-    | 0x100010 => Inv 1 (∃ fb,
-      s R_SP = sp ⊖ 48 /\ s V_MEM64 = mem' fb /\
-      s R_X0 = arg1 /\ s R_X1 = arg2 /\ s R_X2 = arg3
-      )
-      
-    (* loop invariant *)
-    | 0x100020 => Inv 1 (∃ fb k,
-      s R_SP = sp ⊖ 48 /\ s V_MEM64 = mem' fb /\
-      (s R_X19 = mem' fb Ⓠ[k] ) /\
-        s R_X20 = arg1 /\ s R_X21 = arg3
-      )
-
-    (* case-equal, non-null characters found (successful find)*)
-    | 0x100034 => Inv 1 (∃ fb k,
-      s R_SP = sp ⊖ 48 /\ s V_MEM64 = mem' fb /\
-      s R_X19 = mem' fb Ⓠ[k] /\ s R_X20 = arg1 /\ s R_X21 = arg3
-      )
-      
-    (* 0x100048: Just before the "not found" path completes; stack frame and saved registers intact. *)
-    | 0x100048 => Inv 1 (∃ fb,
-      s R_SP = sp ⊖ 48 /\
-      s V_MEM64 = mem' fb /\ (s R_X1 = 0 \/ s R_X19 = 0)
-    )
-
-    (* 0x10004c: After executing `mov x19,#0` (or arriving from cbz), x19 holds the final result value. *)
-    | 0x10004c => Inv 1 (∃ fb n,
-        s R_SP = sp ⊖ 48 /\
-        s V_MEM64 = mem' fb /\
-        s R_X19 = n              (* result in x19 (or 0 if not found) *)
-    )
-
-    (* tfind return site *)
-    | 0x10005c => Post 1 (postcondition s)
-
-    | _ => NoInv
-    end.
-
-  Definition invs1 := make_invs 1 tfind_lo_tfind_armv8 invs.
-  Definition exits1 := make_exits 1 tfind_lo_tfind_armv8 invs.
-  
-End Invariants.
-
-Search "satisfies_all".
 
 Require Import Coq.Lists.List. 
 Require Import Coq.Bool.Bool.
@@ -281,6 +209,88 @@ Proof.
   - right. split; [assumption | unfold sorted_tree in Hsorted; simpl; apply Hsorted with (p1:=q) (p2:=p); assumption].
 Qed.
 
+Section Invariants.
+
+  Variable sp : N          (* initial stack pointer *).
+    
+  Variable mem : memory    (* initial memory state *).
+    
+  Variable arg1 : N        (* tfind: 1st pointer arg (R_X0)
+                              desired index *).
+  Variable arg2 : N        (* tfind: 2nd pointer arg (R_X1)
+                              root node pointer *).
+  Variable arg3 : N        (* tfind: 3rd pointer arg (R_X2)
+                              address of subroutine*).
+  Variable x20 x21 : N     (* R_X20, R_X21 (callee-save regs) *).
+  
+  Variable cmp : cmp_fun.
+
+  Hypothesis Hsorted :
+    sorted_tree 64 LittleE 64 mem arg2 cmp.
+
+  Definition mem' fbytes := setmem 64 LittleE 40 mem (sp ⊖ 48) fbytes.
+
+  Definition postcondition (s:store) :=  
+    ∃ n fb,
+      s V_MEM64 = mem' fb ∧
+      s R_X0 = n.
+  
+  Definition invs T (Inv Post: inv_type T) (NoInv:T) (s:store) (a:addr) : T :=
+    match a with
+    (* tfind entry point *)
+    | 0x100000 => Inv 1 (
+        s R_SP = sp /\ s V_MEM64 = mem /\
+        s R_X0 = arg1 /\ s R_X1 = arg2 /\ s R_X2 = arg3 /\
+        sorted_tree 64 LittleE 64 mem arg2 cmp
+      )
+    
+        (* X1 Parameter Validation *)
+    | 0x100010 => Inv 1 (∃ fb,
+      s R_SP = sp ⊖ 48 /\ s V_MEM64 = mem' fb /\
+      s R_X0 = arg1 /\ s R_X1 = arg2 /\ s R_X2 = arg3
+      )
+      
+    (* loop invariant *)
+    | 0x100020 => Inv 1 (∃ fb k,
+      s R_SP = sp ⊖ 48 /\ s V_MEM64 = mem' fb /\
+      (s R_X19 = mem' fb Ⓠ[k] ) /\
+        s R_X20 = arg1 /\ s R_X21 = arg3 /\
+      sorted_tree 64 LittleE 64 mem arg2 cmp
+      )
+
+    (* case-equal, non-null characters found (successful find)*)
+    | 0x100034 => Inv 1 (∃ fb k,
+      s R_SP = sp ⊖ 48 /\ s V_MEM64 = mem' fb /\
+      s R_X19 = mem' fb Ⓠ[k] /\ s R_X20 = arg1 /\ s R_X21 = arg3
+      )
+      
+    (* 0x100048: Just before the "not found" path completes; stack frame and saved registers intact. *)
+    | 0x100048 => Inv 1 (∃ fb,
+      s R_SP = sp ⊖ 48 /\
+      s V_MEM64 = mem' fb /\ (s R_X1 = 0 \/ s R_X19 = 0)
+    )
+
+    (* 0x10004c: After executing `mov x19,#0` (or arriving from cbz), x19 holds the final result value. *)
+    | 0x10004c => Inv 1 (∃ fb n,
+        s R_SP = sp ⊖ 48 /\
+        s V_MEM64 = mem' fb /\
+        s R_X19 = n              (* result in x19 (or 0 if not found) *)
+    )
+
+    (* tfind return site *)
+    | 0x10005c => Post 1 (postcondition s)
+
+    | _ => NoInv
+    end.
+
+  Definition invs1 := make_invs 1 tfind_lo_tfind_armv8 invs.
+          
+  Definition exits1 := make_exits 1 tfind_lo_tfind_armv8 invs.
+  
+End Invariants.
+
+Search "satisfies_all".
+
 Theorem cset_branch_logic :
    forall s, N.lnot (s R_ZR) 1 mod 2 = 0 \/ N.lnot (s R_ZR) 1 mod 2 = 1.
 Proof.
@@ -315,11 +325,12 @@ Theorem tfind_partial_correctness:
          (MDL: models arm8typctx s)
          (SP: s R_SP = sp) (MEM: s V_MEM64 = mem) (X30: s R_X30 = a')
          (RX0: s R_X0 = arg1) (RX1: s R_X1 = arg2) (RX2: s R_X2 = arg3)
-         (cmp: N -> N -> N -> N)
+         (cmp : cmp_fun)
+          (Hsorted : sorted_tree 64 LittleE 64 mem arg2 cmp)
          (H: good_callee cmp arg3),
           satisfies_all tfind_lo_tfind_armv8 
-                           (invs1  sp mem arg1 arg2 arg3)
-                           (exits1 sp mem arg1 arg2 arg3) ((x',s')::t).
+                           (invs1  sp mem arg1 arg2 arg3 cmp)
+                           (exits1 sp mem arg1 arg2 arg3 cmp) ((x',s')::t).
 
 Proof.
   
@@ -334,14 +345,13 @@ Proof.
   erewrite startof_prefix in ENTRY; try eassumption.
   eapply models_at_invariant; try eassumption. apply welltyped. intro MDL1.
   set (x20 := s R_X20) in *. set (x21 := s R_X21) in *. clearbody x20 x21.
-  clear - PRE MDL1 H cmp. rename t1 into t. rename s1 into s. rename MDL1 into MDL.
+  clear - PRE MDL1 H cmp Hsorted. rename t1 into t. rename s1 into s. rename MDL1 into MDL.
   
   (* Break the proof into cases, one for each internal invariant-point. *)
   destruct_inv 64 PRE.
   
   (* Address 100000: tfind entry point *)
-  (* destruct PRE as (MEM & SP & X0 & X1 & X3).  *)
-  destruct PRE as (SP & MEM & X0 & X1 & X2).
+  destruct PRE as (SP & MEM & X0 & X1 & X2 & HSorted).
   step. step. step. step.
   generalize_frame mem as fb.
   exists fb. psimpl.
@@ -350,23 +360,35 @@ Proof.
   (* Address 100010: tfind Parameter Validation*)
   destruct PRE as (fb & SP & MEM & X0 & X1 & X2).
   step. 
-    (* the root pointer is invalid / 0 *)
-    exists fb. repeat (reflexivity || assumption || split). left. apply N.eqb_eq, BC.
     
-    (* valid root pointer*)
-    step. step. step. exists fb, arg2. repeat (reflexivity || assumption || split).
+  (* the root pointer is invalid / 0 *)
+  exists fb. 
+  repeat (reflexivity || assumption || split). 
+  left. apply N.eqb_eq, BC.
     
+  (* valid root pointer*)
+  step. step. step. 
+  exists fb, arg2. 
+  repeat (reflexivity || assumption || split).
   
   (* Address 100020: tfind main Loop*)  
-  destruct PRE as (fb & k & SP & MEM & X19 & X20 & X21).
+  destruct PRE as (fb & k & SP & MEM & X19 & X20 & X21 & HSorted).
   step.
   
-    (* invalid pointer at current node*)
-  + exists fb. repeat (reflexivity || assumption || split). right. apply N.eqb_eq, BC.
+  (* invalid pointer at current node*)
+  + exists fb. 
+  repeat (reflexivity || assumption || split). 
+  right. apply N.eqb_eq, BC.
   
     (* valid node main loop section with BLR call *)
-  + step. step. step. apply H. intros. unfold callee_postcondition in H0.
-  step. exists fb, k. repeat (destruct H2 || destruct H0 || destruct H1). repeat (split || assumption).
+  + step. step. step. 
+  apply H. 
+  intros. 
+  unfold callee_postcondition in H0.
+  step. 
+  exists fb, k. 
+  repeat (destruct H2 || destruct H0 || destruct H1). 
+  repeat (split || assumption).
   
   (* Address 100034: case-equal, non-null characters found (successful find)*)
   + destruct PRE as (fb & k & SP & MEM & X19 & X20 & X21).
@@ -374,15 +396,27 @@ Proof.
   exists fb, (mem' sp mem fb Ⓠ[ k ]).
   repeat (assumption || reflexivity || split).
   step. step. step. step.
-  exists fb. eexists.
+  exists fb. 
+  eexists.
   repeat (assumption || reflexivity || split).
   
   
   (* Address 100048: Just before the "not found" path completes; stack frame and saved registers intact. *)
   + destruct PRE as (fb & SP & MEM & zero).
-  step. exists fb, 0. repeat (assumption || reflexivity || split).
+  step. 
+  exists fb, 0. 
+  repeat (assumption || reflexivity || split).
   
-  + destruct PRE as ( fb & addr & SP & MEM & X19).
+  (* Address 10004c *)
+  + destruct PRE as (fb & SP & MEM & zero).
   step. step. step. step.
-      
+  
+  
+  destruct zero as (HMEM & HX19).
+  exists SP, fb.
+  split.
+  assumption.
+  assumption.
+  
+  
 Qed.
